raft-proofs/RaftRefinementProof.v
@@ -202,6 +202,221 @@ Section RaftRefinementProof.
     - eapply_prop refined_raft_net_invariant_do_generic_server; eauto.
   Qed.
 
+  Lemma refined_raft_invariant_handle_message' P :
+    forall xs p ys net st' ps' gd d l,
+      refined_raft_net_invariant_append_entries' P ->
+      refined_raft_net_invariant_append_entries_reply' P ->
+      refined_raft_net_invariant_request_vote' P ->
+      refined_raft_net_invariant_request_vote_reply' P ->
+      handleMessage (pSrc p) (pDst p) (pBody p) (snd (nwState net (pDst p))) = (d, l) ->
+      update_elections_data_net (pDst p) (pSrc p) (pBody p) (nwState net (pDst p)) = gd ->
+      P net ->
+      refined_raft_intermediate_reachable net ->
+      refined_raft_intermediate_reachable (mkNetwork ps' st') ->
+      nwPackets net = xs ++ p :: ys ->
+      (forall h, st' h = update (nwState net) (pDst p) (gd, d) h) ->
+      (forall p', In p' ps' -> In p' (xs ++ ys) \/
+                             In p' (send_packets (pDst p) l)) ->
+      P (mkNetwork ps' st').
+  Proof.
+    intros.
+    unfold handleMessage, update_elections_data_net in *.
+    break_match; repeat break_let; repeat find_inversion;
+    [eapply_prop refined_raft_net_invariant_request_vote'|
+     eapply_prop refined_raft_net_invariant_request_vote_reply'|
+     eapply_prop refined_raft_net_invariant_append_entries'|
+     eapply_prop refined_raft_net_invariant_append_entries_reply']; eauto;
+    unfold send_packets in *; simpl in *; intros; subst; auto; find_apply_hyp_hyp; intuition.
+  Qed.
+
+  Lemma refined_raft_invariant_handle_input' P :
+    forall h inp net st' ps' gd out d l,
+      refined_raft_net_invariant_timeout' P ->
+      refined_raft_net_invariant_client_request' P ->
+      handleInput h inp (snd (nwState net h)) = (out, d, l) ->
+      update_elections_data_input h inp (nwState net h) = gd ->
+      P net ->
+      refined_raft_intermediate_reachable net ->
+      refined_raft_intermediate_reachable (mkNetwork ps' st') ->
+      (forall h', st' h' = update (nwState net) h (gd, d) h') ->
+      (forall p', In p' ps' -> In p' (nwPackets net) \/
+                         In p' (send_packets h l)) ->
+      P (mkNetwork ps' st').
+  Proof.
+    intros.
+    unfold handleInput, update_elections_data_input in *.
+    break_match; repeat break_let; repeat find_inversion;
+    [eapply_prop refined_raft_net_invariant_timeout'|
+     eapply_prop refined_raft_net_invariant_client_request']; eauto; subst; auto.
+  Qed.
+
+  Theorem refined_raft_net_invariant' :
+    forall P net,
+      refined_raft_net_invariant_init P ->
+      refined_raft_net_invariant_client_request' P ->
+      refined_raft_net_invariant_timeout' P ->
+      refined_raft_net_invariant_append_entries' P ->
+      refined_raft_net_invariant_append_entries_reply' P ->
+      refined_raft_net_invariant_request_vote' P ->
+      refined_raft_net_invariant_request_vote_reply' P ->
+      refined_raft_net_invariant_do_leader' P ->
+      refined_raft_net_invariant_do_generic_server' P ->
+      refined_raft_net_invariant_state_same_packet_subset P ->
+      refined_raft_net_invariant_reboot' P ->
+      refined_raft_intermediate_reachable net ->
+      P net.
+  Proof.
+    intros.
+    induction H10.
+    - intuition.
+    -  match goal with [H : step_f _ _ _ |- _ ] => invcs H end.
+       + match goal with 
+         | [ H : refined_raft_intermediate_reachable _ |- _ ?x ] => 
+           assert (refined_raft_intermediate_reachable x) as Hpost
+                  by (eapply RRIR_step_f; eauto; eapply SF_deliver; eauto)
+         
+         end.
+         unfold refined_net_handlers in *. simpl in *.
+         unfold RaftNetHandler, update_elections_data_net in *.
+         repeat break_let.
+         repeat find_inversion.
+         match goal with 
+         | [ H : refined_raft_intermediate_reachable ?net, H' : context [net]  |- _ ] => 
+           match type of H' with
+           | refined_raft_intermediate_reachable _ => move H after H'
+           end
+         end.
+         assert
+           (refined_raft_intermediate_reachable
+              {|
+                nwPackets := (xs ++ ys) ++ send_packets (pDst p) l2;
+                nwState := update (nwState net) (pDst p)
+                                  (update_elections_data_net (pDst p)
+                                                             (pSrc p)
+                                                             (pBody p)
+                                                             (nwState net (pDst p)), r0) |})
+           by (eapply RRIR_handleMessage; eauto; in_crush).
+         assert
+           (refined_raft_intermediate_reachable
+              {|
+                nwPackets := ((xs ++ ys)
+                                ++ send_packets (pDst p) l2)
+                               ++ send_packets (pDst p) l3 ;
+            nwState := update
+                         (nwState
+                            {|
+                              nwPackets := (xs ++ ys) ++ send_packets (pDst p) l2;
+                              nwState := update (nwState net)
+                                                (pDst p)
+                                                (update_elections_data_net
+                                                   (pDst p) (pSrc p)
+                                                   (pBody p) (nwState net (pDst p)), r0) |})
+                         (pDst p)
+                         (update_elections_data_net (pDst p)
+                                                    (pSrc p) (pBody p) (nwState net (pDst p)), r1) |})
+           by
+             (eapply RRIR_doGenericServer; eauto;
+              [simpl in *; break_if; try congruence; eauto| in_crush]).
+         eapply_prop refined_raft_net_invariant_do_leader'. eauto.
+         eapply_prop refined_raft_net_invariant_do_generic_server'. eauto.
+         eapply refined_raft_invariant_handle_message' with (P := P); auto.
+         eauto. eauto.   auto. eauto.  eauto. eauto using in_app_or. auto.
+         eauto.
+         simpl. break_if; intuition eauto.
+         eauto.
+         simpl. eapply in_app_or. auto. auto.
+         simpl. break_if; eauto; congruence.
+         simpl. intros.
+         break_if; subst;
+         repeat rewrite update_same by auto;
+         repeat rewrite update_neq by auto; auto.
+         simpl. in_crush.
+       + match goal with 
+         | [ H : refined_raft_intermediate_reachable _ |- _ ?x ] => 
+           assert (refined_raft_intermediate_reachable x) as Hpost
+               by (eapply RRIR_step_f; eauto; eapply SF_input; eauto)
+         end.
+         unfold refined_input_handlers in *. simpl in *.
+         unfold RaftInputHandler, update_elections_data_input in *. repeat break_let.
+         repeat find_inversion.
+         match goal with 
+         | [ H : refined_raft_intermediate_reachable ?net, H' : context [net]  |- _ ] => 
+           match type of H' with
+           | refined_raft_intermediate_reachable _ => move H after H'
+           end
+         end.                    
+
+         assert
+           (refined_raft_intermediate_reachable
+              {|
+                nwPackets := nwPackets net ++ send_packets h l2;
+                nwState := update (nwState net) h
+                                  (update_elections_data_input h
+                                                               inp
+                                                               (nwState net h), r0) |})
+           by (eapply RRIR_handleInput; eauto; in_crush).
+         assert
+           (refined_raft_intermediate_reachable
+              {|
+                nwPackets := (nwPackets net
+                                ++ send_packets h l2)
+                               ++ send_packets h l4 ;
+            nwState := update
+                         (nwState
+                            {|
+                              nwPackets := nwPackets net ++ send_packets h l2;
+                              nwState := update (nwState net)
+                                                h
+                                                (update_elections_data_input h inp
+                                                                             (nwState net h), r0) |})
+                         h
+                         (update_elections_data_input h inp (nwState net h), r1) |})
+           by
+             (eapply RRIR_doGenericServer; eauto;
+              [simpl in *; break_if; try congruence; eauto| in_crush]).
+         eapply_prop refined_raft_net_invariant_do_leader'. eauto.
+         eapply_prop refined_raft_net_invariant_do_generic_server'. eauto.
+         eapply refined_raft_invariant_handle_input' with (P := P); auto. 
+         eauto. all:auto. all: eauto. eauto using in_app_or. 
+         simpl. break_if; intuition eauto.
+         eauto.
+         simpl. eapply in_app_or.
+         auto.
+         simpl. break_if; eauto; congruence.
+         simpl. intros.
+         break_if; subst;
+         repeat rewrite update_same by auto;
+         repeat rewrite update_neq by auto; auto.
+         simpl. unfold send_packets.  intros. in_crush.
+       + match goal with
+           | [ H : nwPackets ?net = _ |- _ {| nwPackets := ?ps ; nwState := ?st |} ] =>
+             assert (forall p, In p (nwPackets {| nwPackets := ps ; nwState := st |}) ->
+                          In p (nwPackets net)) by (intros; simpl in *; find_rewrite; in_crush)
+         end.
+         eapply_prop refined_raft_net_invariant_state_same_packet_subset; [|eauto|idtac|];
+         eauto.
+       + match goal with
+           | [ H : nwPackets ?net = _ |- _ {| nwPackets := ?ps ; nwState := ?st |} ] =>
+             assert (forall p, In p (nwPackets {| nwPackets := ps ; nwState := st |}) ->
+                          In p (nwPackets net)) by (intros; simpl in *; find_rewrite; in_crush)
+         end.
+         eapply_prop refined_raft_net_invariant_state_same_packet_subset; [|eauto|idtac|];
+         eauto.
+       + auto.
+       + eapply_prop refined_raft_net_invariant_reboot'; eauto;
+         intros; simpl in *; repeat break_if; intuition; subst; intuition eauto.
+         * econstructor. eauto. eapply SF_reboot; eauto.
+         * destruct (nwState net h); auto.
+    - eapply refined_raft_invariant_handle_input'; eauto.
+      eapply RRIR_handleInput; eauto.
+    - eapply refined_raft_invariant_handle_message'; eauto.
+      eapply RRIR_handleMessage; eauto.
+    - eapply_prop refined_raft_net_invariant_do_leader'; eauto.
+      eapply RRIR_doLeader; eauto.
+    - eapply_prop refined_raft_net_invariant_do_generic_server'; eauto.
+      eapply RRIR_doGenericServer; eauto.
+  Qed.
+
   Require Import FunctionalExtensionality.
 
   Ltac workhorse :=
@@ -416,6 +631,7 @@ Section RaftRefinementProof.
   Proof.
     split.
     - exact refined_raft_net_invariant.
+    - exact refined_raft_net_invariant'.
     - exact lift_prop.
     - exact lower_prop.
     - exact deghost_spec.
